src/examples/mulc.v
@@ -99,6 +99,9 @@ Proof.
   apply (ltn_addl (odd m)) in LT3.
   by rewrite -(ltn_add2l (odd m)).
 
+  autorewrite with push_at. 
+  unhideFlag OF => oF. unhideFlag SF => sF. unhideFlag ZF => zF. 
+  unhideFlag CF => cF. unhideFlag PF => pF. 
   case ODD: (odd m); first case ZERO: (c == 0);
   do ?basic apply * => //.
 
@@ -109,10 +112,10 @@ Proof.
   (* ADD r1, r2 *)
   rewrite (eqP ZERO).  rewrite expn0 muln1 expn1.
   rewrite muln2. rewrite -{2}(odd_double_half m) ODD. rewrite /stateIs mulB_addn mulB1. rewrite -> addBA.
-  sbazooka.
+  sbazooka. 
 
-  rewrite (eqP ZERO) add0n in LT1. sbazooka. ssimpl. rewrite add1n.
-
+  by rewrite (eqP ZERO) add0n in LT1.
+  
   (* c is not 0 *)
 
   (* SHL r2, c *)
@@ -121,7 +124,7 @@ Proof.
 
   rewrite expn1 -{2}(odd_double_half m) ODD. rewrite muln2. rewrite -addBA.
   rewrite mulnDl mul1n. rewrite mulB_addn. rewrite mulnC.
-  rewrite shlB_mul2exp mulB_muln /stateIs. sbazooka.
+  rewrite shlB_mul2exp mulB_muln /stateIs. by ssimpl.  
 
   rewrite add1n. rewrite -addn1 addnA addn1 addnC in LT1.
   apply (ltn_addr c) in LT1. by rewrite -(ltn_add2r c).
@@ -168,14 +171,11 @@ autorewrite with push_at.
 case EQ2: (m == 2); last case EQ4: (m == 4); last case EQ8: (m == 8);
 do ?basic apply * => //.
 
-rewrite /eval.computeIxAdr/eval.computeAdr/eval.scaleBy/eval.computeDisplacement shlB_asMul (eqP EQ2).
-rewrite -> addB0. by ssimpl.
+rewrite shlB_asMul (eqP EQ2). by ssimpl.
 
-rewrite /eval.computeIxAdr/eval.computeAdr/eval.scaleBy/eval.computeDisplacement !shlB_asMul (eqP EQ4) -mulB_muln.
-rewrite -> addB0. change (2*2) with 4. by ssimpl.
+rewrite !shlB_asMul (eqP EQ4) -mulB_muln. change (2*2) with 4. by ssimpl.
 
-rewrite /eval.computeIxAdr/eval.computeAdr/eval.scaleBy/eval.computeDisplacement !shlB_asMul (eqP EQ8) -!mulB_muln.
-rewrite -> addB0. change (2*_) with 8. by ssimpl.
+rewrite !shlB_asMul (eqP EQ8) -!mulB_muln. change (2*_) with 8. by ssimpl.
 
 by rewrite /stateIs expn0 muln1.
 Qed.
@@ -229,6 +229,9 @@ Proof.
   apply (ltn_addl (odd m)) in LT3.
   by rewrite -(ltn_add2l (odd m)).
 
+  autorewrite with push_at. 
+  unhideFlag OF => oF. unhideFlag SF => sF. unhideFlag ZF => zF. 
+  unhideFlag CF => cF. unhideFlag PF => pF. 
   case ODD: (odd m); first destruct c as [|[|[|[|]]]];
   do ?basic apply * => //.
 
@@ -245,7 +248,7 @@ Proof.
 
   rewrite expn1 -{2}(odd_double_half m) ODD. rewrite muln2. rewrite -addBA.
   replace (2^2) with (2*2) by done. rewrite mulnA. rewrite -mulB_addn. rewrite !muln2.
-  rewrite -(odd_double_half m). rewrite /eval.computeAdr/eval.computeDisplacement. rewrite -> addB0. 
+  rewrite -(odd_double_half m). 
   by rewrite ODD mulB_addn.
 
   (* c is 2 *)
@@ -258,12 +261,11 @@ Proof.
   replace (2+m./2 * 2 *2) with (true*2 + m./2 * 2 * 2) by done.
   rewrite -mulnDl.
   rewrite -ODD. rewrite !muln2. rewrite -> (odd_double_half m).
-  rewrite -!muln2 /stateIs. rewrite /eval.computeAdr/eval.computeDisplacement. rewrite -> addB0. 
+  rewrite -!muln2 /stateIs. 
   by rewrite mulnA.
 
   (* c is 3 *)
-  rewrite /eval.scaleBy/eval.computeIxAdr/eval.computeAdr/eval.computeDisplacement !shlB_asMul.
-  rewrite -> addB0.
+  rewrite !shlB_asMul.
   rewrite -addBA. rewrite <-!mulBA. rewrite <- (mulBDr w).
   rewrite 4!expnS expn0 muln1 mulnA.
   rewrite 2!fromNat_mulBn. rewrite fromNat_addBn. rewrite 2!mulnA. rewrite -mulnDl.
