src/x86/addr.v
@@ -8,9 +8,12 @@ Set Implicit Arguments.
 Unset Strict Implicit.
 Import Prenex Implicits.
 
-(* In 64-bit mode there are two address sizes: 32-bit and 64-bit *)
+(* In 64-bit mode there are two sizes for effective addresses: 32-bit and 64-bit *)
+(* This offset is added to the 64-bit segment base (0, except for FS and GS) *)
 Inductive AdSize := AdSize4 | AdSize8.
 Definition adSizeToOpSize a := match a with AdSize4 => OpSize4 | AdSize8 => OpSize8 end.
+
+(* Address offset, before widening and adding to segment base *)
 Definition ADR a := VWORD (adSizeToOpSize a).
 Identity Coercion ADRtoVWORD : ADR >-> VWORD.
 
@@ -18,6 +21,7 @@ Identity Coercion ADRtoVWORD : ADR >-> VWORD.
    @TODO: what do we do about canonical addressing (see 3.3.7.1)? *)
 Definition naddrBits := n64.
 
+(* Logical address, after adding in segment base *)
 Definition ADDR := QWORD.
 Identity Coercion ADDRtoQWORD : ADDR >-> QWORD.
 
@@ -27,7 +31,12 @@ Identity Coercion ADDRCursortoQWORDCUrsor : ADDRCursor >-> QWORDCursor.
 Definition (*Coercion*) ADDRtoADDRCursor (x:ADDR) : ADDRCursor := mkCursor x.
 Definition (*Coercion*) ADRtoADDR a  :=
   match a return ADR a -> ADDR with 
-  | AdSize4 => fun x => zeroExtend 32 x
+  | AdSize4 => fun x => zeroExtend n32 x
+  | AdSize8 => fun x => x
+  end.
+Definition (*Coercion*) ADDRtoADR a  :=
+  match a return ADDR -> ADR a with 
+  | AdSize4 => fun x => low n32 x
   | AdSize8 => fun x => x
   end.
 
