src/x86/instrrules/and.v
@@ -3,60 +3,16 @@ Require Import x86proved.x86.instrrules.core.
 Import x86.instrrules.core.instrruleconfig.
 
 (** ** Generic AND *)
-
-(** ** AND r1, [r2 + offset] *)
-(*
-Example AND_RM_rule (pbase:DWORD) (r1 r2:GPReg32) v1 (v2:DWORD) (offset:nat) :
-  |-- basic (r1~=v1 ** OSZCP?)
-            (AND r1, [r2 + offset]) empOP
-            (let v:= andB v1 v2 in r1~=v ** OSZCP false (msb v) (v == #0) false (lsb v))
-      @ (r2 ~= pbase ** adrToADDR (a:=AdSize4) (computeAddr (a:=AdSize4) pbase offset) :-> v2).
-Proof.
-do_instrrule_triple. 
-Qed.
-*)
-
-Require Import x86proved.monad monadinst eval. 
-Lemma AND_rule sz (ds:DstSrc sz) (v1: VWORD sz) :
+Lemma AND_rule s (ds:DstSrc s) (v1: VWORD s) :
    |-- specAtDstSrc ds (fun D v2 =>
        basic (D v1 ** OSZCP?)
              (BOP _ OP_AND ds) empOP
              (let v := andB v1 v2 in
               D v ** OSZCP false (msb v) (v == #0) false (lsb v))).
-Proof. do_instrrule_triple. Qed.
+Proof. destruct ds; do_instrrule_triple. Qed. 
 
 (** We make this rule an instance of the typeclass, and leave
     unfolding things like [specAtDstSrc] to the getter tactic
     [get_instrrule_of]. *)
-Global Instance: forall sz (ds : DstSrc sz), instrrule (BOP sz OP_AND ds) := @AND_rule.
+Global Instance: forall s (ds : DstSrc s), instrrule (BOP _ OP_AND ds) := @AND_rule.
 
-(* Our original formalization defined a bunch of more specific rules such as the following.
-   These are now simple corollaries of the general rule above i.e. "examples" *)
-
-(** ** AND r1, r2 *)
-Example AND_RR_rule (r1 r2:GPReg32) v1 (v2:DWORD) :
-  |-- basic (r1~=v1 ** r2 ~= v2 ** OSZCP?)
-            (AND r1, r2) empOP
-            (let v := andB v1 v2 in r1~=v ** r2 ~= v2 **
-             OSZCP false (msb v) (v == #0) false (lsb v)).
-Proof. basic apply *. Qed.
-
-(** ** AND r1, [r2 + offset] *)
-Example AND_RM_rule (pbase:DWORD) (r1 r2:GPReg32) v1 (v2:DWORD) (offset:nat) :
-  |-- basic (r1~=v1 ** OSZCP?)
-            (AND r1, [r2 + offset]) empOP
-            (let v:= andB v1 v2 in r1~=v ** OSZCP false (msb v) (v == #0) false (lsb v))
-      @ (r2 ~= pbase ** (eval.computeAddr (a:=AdSize4) pbase offset) :-> v2).
-Proof. autorewrite with push_at. basic apply *. Qed.
-
-Example AND_RM_ruleNoFlags (pd:DWORD) (r1 r2:GPReg32) v1 (v2:DWORD) (offset:nat):
-  |-- basic (r1~=v1) (AND r1, [r2 + offset]) empOP (r1~=andB v1 v2)
-             @ (r2 ~= pd ** eval.computeAddr (a:=AdSize4) pd offset :-> v2 ** OSZCP?).
-Proof. autorewrite with push_at. basic apply *. Qed.
-
-(** ** AND r, v *)
-Example AND_RI_rule (r:GPReg32) v1 (v2:DWORD) :
-  |-- basic (r~=v1 ** OSZCP?)
-            (AND r, v2) empOP
-            (let v:= andB v1 v2 in r~=v ** OSZCP false (msb v) (v == #0) false (lsb v)).
-Proof. basic apply *. Qed.
