src/x86/instrrules/neg.v
@@ -3,14 +3,14 @@ Require Import x86proved.x86.instrrules.core.
 Import x86.instrrules.core.instrruleconfig.
 
 (** Special case for negation *)
-Lemma NEG_R_rule s (r:GPReg s) (v:VWORD s) :
+Lemma NEG_rule s (src: RegMem s) (v:VWORD s) :
   let w := negB v in
-  |-- basic
-    (r ~= v ** OSZCP?) (NEG r) empOP
-    (r ~= w ** OSZCP (msb v!=msb w) (msb w) (w == #0) (v != #0) (lsb w)).
-Proof. destruct s; do_instrrule_triple. Qed.
+  |-- specAtRegMemDst src (fun V =>
+    basic (V v ** OSZCP?) (UOP s OP_NEG src) empOP
+          (V w ** OSZCP (msb v!=msb w) (msb w) (w == #0) (v != #0) (lsb w))).
+Proof. do_instrrule_triple. Qed.
 
 (** We make this rule an instance of the typeclass, and leave
     unfolding things like [specAtDstSrc] to the getter tactic
     [get_instrrule_of]. *)
-Global Instance: forall s (r : GPReg s), instrrule (NEG r) := @NEG_R_rule.
+Global Instance: forall s (src : RegMem s), instrrule (UOP _ OP_NOT src) := @NEG_rule.
