src/x86/instrrules/not.v
@@ -11,19 +11,3 @@ Proof. do_instrrule_triple. Qed.
     [get_instrrule_of]. *)
 Global Instance: forall d (src : RegMem d), instrrule (UOP d OP_NOT src) := @NOT_rule.
 
-
-(** Special case for not *)
-Lemma NOT_R_rule (r:GPReg32) (v:DWORD):
-  |-- basic (r~=v) (NOT r) empOP (r~=invB v).
-Proof. basic apply *. Qed.
-
-(*
-(* BUG: default for NOT syntax on pointers appears to be dword size. *)
-Corollary NOT_M_rule (r:GPReg64) (offset:nat) (pbase:ADDR) (v:QWORD):
-  |-- basic (r~=pbase ** eval.computeAddr (a:=AdSize8) pbase offset :-> v) (NOT [r + offset]) empOP
-            (r~=pbase ** eval.computeAddr (a:=AdSize8) pbase offset :-> invB v).
-Proof. (*attempt basic apply *. *)
- attempt basic apply (NOT_rule (d:=OpSize8)).  *. setoid_rewrite empSPR. Set Printing All. Show. 
-(* OK, we seem to have a default points-to of size 4 here. Why? *)
-reflexivity. ssimpl. Set Printing Coercions. sbazooka.  Show. ssimpl. Qed.
-*)
