src/x86/instrrules/pop.v
@@ -13,26 +13,3 @@ Proof. do_instrrule_triple. Qed.
     unfolding things like [specAtDstSrc] to the getter tactic
     [get_instrrule_of]. *)
 Global Instance: forall (rm : RegMem _), instrrule (POP rm) := @POP_rule.
-
-
-(** ** POP r *)
-Corollary POP_R_rule (r:GPReg64) (sp oldv v:QWORD) :
-  |-- basic (r ~= oldv ** RSP ~= sp    ** sp:->v) (POP (RegMemR OpSize8 r)) empOP
-            (r ~= v    ** RSP ~= sp+#8 ** sp:->v).
-Proof. basic apply *. Qed.
-
-(** ** POP [r + offset] *)
-(*Corollary POP_M_rule (r:GPReg64) (offset:nat) (sp oldv v pbase:QWORD) :
-  |-- basic (r ~= pbase ** pbase +# offset :-> oldv ** RSP ~= sp ** sp :-> v)
-            (POP [r + offset]) empOP
-            (r ~= pbase ** pbase +# offset :-> v ** RSP ~= sp+#8 ** sp :-> v).
-
-Proof. basic apply *. Qed.
-
-(** ** POP [r] *)
-Corollary POP_M0_rule (r: GPReg32) (sp oldv v pbase:DWORD) :
-  |-- basic (r ~= pbase ** pbase :-> oldv ** ESP ~= sp    ** sp :-> v)
-            (POP [r]) empOP
-            (r ~= pbase ** pbase :-> v    ** ESP ~= sp+#4 ** sp :-> v).
-Proof. basic apply *. Qed.
-*)
