src/x86/instrrules/test.v
@@ -8,10 +8,12 @@ Lemma TEST_self_rule s (r:GPReg s) (v:VWORD s) :
   |-- basic (r ~= v ** OSZCP?) (TEST r, r) empOP
             (r ~= v ** OSZCP false (msb v) (v == #0) false (lsb v)).
 Proof.
-  do_instrrule (instrrule_triple_bazooka; rewrite andBB; instrrule_triple_bazooka).
+  Hint Rewrite andBB : triple.
+  do_instrrule_triple.
 Qed.
 
 (** We make this rule an instance of the typeclass, and leave
     unfolding things like [specAtDstSrc] to the getter tactic
     [get_instrrule_of]. *)
 Global Instance: forall s (r : GPReg s), instrrule (TEST r, r) := @TEST_self_rule.
+
